LeanMove/Lang/PrettyPrint.lean
@@ -48,10 +48,13 @@ def ppBorrowingKind : BorrowingKind → String
   | .siteBorrowImm => ".siteBorrowImm"
   | .siteBorrowMut => ".siteBorrowMut"
 
+def ppIntType : IntType → String
+  | .u8 => "u8" | .u16 => "u16" | .u32 => "u32"
+  | .u64 => "u64" | .u128 => "u128" | .u256 => "u256"
+
 mutual
   partial def ppBasicMoveType : BasicMoveType → String
-    | .u64 => ".u64"
-    | .u8 => ".u8"
+    | .int w => s!".{ppIntType w}"
     | .tbool => ".tbool"
     | .tunit => ".tunit"
     | .trecord m => s!".trecord {ppFieldMap m}"
@@ -111,7 +114,7 @@ def ppExprMacro : Expr → String
   | .usage (.move v) => s!"move {ppVar v}"
   | .usage (.borrowImm v) => s!"&{ppVar v}"
   | .usage (.borrowMut v) => s!"&mut {ppVar v}"
-  | .intLit n => s!"#{n}"
+  | .intLit n w => s!"#{n}{ppIntType w}"
   | .borrowField src bt f =>
     s!"borrowField({ppSite src}, {ppBasicMoveType bt}, {ppField f})"
   | .borrowMutField src bt f =>
